working on addEdgeLemm

examples/logic/ltl/concrRepScript.sml
@@ -8,15 +8,16 @@ val _ = monadsyntax.temp_add_monadsyntax();
 val _ = overload_on("monad_bind",``OPTION_BIND``);
 
 val _ = Datatype`
-  nodeLabelAA = <| frml : α ltl_frml ;
-                   is_final : bool
-                 |>`;
-
-val _ = Datatype`
   edgeLabelAA = <| edge_grp : num ;
                    pos_lab : (α list) ;
                    neg_lab : (α list)
                  |>`;
+
+val _ = Datatype`
+nodeLabelAA = <| frml : α ltl_frml ;
+                 is_final : bool ;
+                 true_labels : (α edgeLabelAA) list
+               |>`;
 
 val _ = Datatype`
   concrAA = <| graph : (α nodeLabelAA, α edgeLabelAA) gfg ;
@@ -59,19 +60,28 @@ val concr2AbstractEdge_def = Define`
 
 val extractTrans_def = Define`
   extractTrans graph s =
-     let sucs = OPTION_TO_LIST
-                 (do node <- findNode (λ(n,l). l.frml = s) graph ;
-                     lookup node graph.followers
-                  od
-                 )
-     in { edge | ?label.
+     let sucs =
+            OPTION_TO_LIST
+               (do (nId,nodeLabel) <- findNode (λ(n,l). l.frml = s) graph ;
+                   lookup nId graph.followers
+                od
+               )
+     in let trueLabels =
+              OPTION_TO_LIST
+              (do (nId, nodeLabel) <- findNode (λ(n,l). l.frml = s) graph ;
+                  SOME nodeLabel.true_labels
+               od
+              )
+     in { edge | ?label. 0 < label.edge_grp
+                 ∧
                  let labelSucs =
                      { suc.frml
                      | ?sucId. MEM (label,sucId) sucs
                         ∧ SOME suc = lookup sucId graph.nodeInfo
                      }
                  in (edge = (label.edge_grp, label.pos_lab,
-                             label.neg_lab, labelSucs)) }`;
+                             label.neg_lab, labelSucs)) }
+      ∪ { (0,l.pos_lab,l.neg_lab,{}) | MEM l trueLabels }`;
 
 val concr2AbstrAA = Define`
   concr2AbstrAA (concrAA g init prop) =
@@ -82,6 +92,98 @@ val concr2AbstrAA = Define`
         (POW (LIST_TO_SET prop))
         (\f. IMAGE (λ(i,p,n,e). (transformLabel (props f) p n,e))
                    (extractTrans g f))`;
+
+val graphStatesWithId_def = Define`
+  graphStatesWithId g =
+        MAP (λ(id,label). (id, label.frml)) (toAList g.nodeInfo)`;
+
+val unique_node_formula_def = Define`
+  unique_node_formula g =
+   ∀id h.
+    MEM (id,h) (graphStatesWithId g) ⇒
+     ∀oId. MEM (oId,h) (graphStatesWithId g) ⇒ (id = oId)`;
+
+val UNIQUE_NODE_FORM_LEMM = store_thm
+  ("UNIQUE_NODE_FORM_LEMM",
+   ``!g f. unique_node_formula g
+             ==> (OPTION_MAP (λ(id,label). (id,label.frml))
+                      (findNode (λ(n,l). l.frml = f) g)
+                   = FIND (λa. SND a = f) (graphStatesWithId g))``,
+   rpt strip_tac >> fs[findNode_def,graphStatesWithId_def]
+   >> Cases_on
+       `FIND (λa. SND a = f)
+             (MAP (λ(id,label). (id,label.frml))
+                  (toAList g.nodeInfo))`
+   >- (fs[]
+       >> `!x. MEM x (MAP (λ(id,label). (id,label.frml)) (toAList g.nodeInfo))
+               ==> ~((λa. SND a = f) x)` by (
+          Q.HO_MATCH_ABBREV_TAC `!x. MEM x L ==> ~P x`
+          >> rpt strip_tac
+          >> `?z. FIND P L = SOME z` by metis_tac[FIND_LEMM]
+          >> fs[]
+        )
+       >> Q.HO_MATCH_ABBREV_TAC `FIND P L = NONE`
+       >> `!x. MEM x L ==> ~P x` by (
+          rpt strip_tac
+          >> first_x_assum
+               (qspec_then `(λ(id,label). (id,label.frml)) x` mp_tac)
+          >> fs[MEM_MAP] >> rpt strip_tac
+          >- (qunabbrev_tac `P` >> fs[] >> metis_tac[])
+          >- (qunabbrev_tac `P` >> Cases_on `x` >> fs[])
+        )
+       >> `!x. ~(FIND P L = SOME x)` by (
+            rpt strip_tac >> metis_tac[FIND_LEMM2]
+        )
+       >> Cases_on `FIND P L` >> fs[]
+      )
+   >- (`MEM x (MAP
+                (λ(id,label). (id,label.frml))
+                (toAList g.nodeInfo))
+      ∧ (λa. SND a = f) x`
+         by (Q.HO_MATCH_ABBREV_TAC `MEM x L ∧ P x` >> metis_tac[FIND_LEMM2])
+       >> `?y.(FIND (λ(n,l). l.frml = f) (toAList g.nodeInfo)) = SOME y
+         ∧ (λ(id,label). (id,label.frml)) y = x` suffices_by (
+          fs[] >> rpt strip_tac >> fs[]
+       )
+       >> fs[unique_node_formula_def,graphStatesWithId_def]
+       >> `?z. MEM z (toAList g.nodeInfo) ∧ (λ(n,l). l.frml = f) z`
+          by (fs[MEM_MAP] >> qexists_tac `y` >> Cases_on `y` >> fs[] >> rw[])
+       >> `?a. FIND (λ(n,l). l.frml = f) (toAList g.nodeInfo) = SOME a`
+          by metis_tac[FIND_LEMM]
+       >> qexists_tac `a` >> fs[] >> Cases_on `a` >> Cases_on `x`
+       >> fs[] >> first_x_assum (qspec_then `q'` mp_tac) >> strip_tac
+       >> first_x_assum (qspec_then `f` mp_tac) >> simp[] >> strip_tac
+       >> first_x_assum (qspec_then `q` mp_tac) >> strip_tac
+       >> `MEM (q,r) (toAList g.nodeInfo) ∧ (λ(n,l). l.frml = f) (q,r)`
+          by metis_tac[FIND_LEMM2] >> fs[]
+       >> `MEM (q,f)
+            (MAP (λ(id,label). (id,label.frml)) (toAList g.nodeInfo))` by (
+          simp[MEM_MAP] >> qexists_tac `(q,r)` >> fs[]
+       )
+       >> metis_tac[]
+      )
+  );
+
+val UNIQUE_NODE_FORM_LEMM2 = store_thm
+  ("UNIQUE_NODE_FORM_LEMM",
+   ``!g. unique_node_formula g
+         ==> (!f x. (SND x = f) ∧ MEM x (graphStatesWithId g)
+               ==> !y. (SND y = f) ∧ MEM y (graphStatesWithId g)
+                    ==> (x = y))``,
+   rpt strip_tac >> fs[graphStatesWithId_def,unique_node_formula_def]
+   >> Cases_on `x` >> Cases_on `y`
+   >> first_x_assum (qspec_then `q` mp_tac) >> rpt strip_tac
+   >> first_x_assum (qspec_then `f` mp_tac)
+   >> `MEM (q,f)
+         (MAP (λ(id,label). (id,label.frml)) (toAList g.nodeInfo))`
+      by (fs[MEM_MAP] >> qexists_tac `y` >> Cases_on `y` >> fs[])
+   >> simp[] >> strip_tac
+   >> first_x_assum (qspec_then `q'` mp_tac)
+   >> `MEM (q',f) (MAP (λ(id,label). (id,label.frml)) (toAList g.nodeInfo))`
+      by (fs[MEM_MAP] >> qexists_tac `y'` >> Cases_on `y'` >> fs[])
+   >> simp[] >> fs[]
+  );
+
 
 val graphStates_def = Define
  `graphStates g = MAP ((\l. l.frml) o SND) (toAList g.nodeInfo)`;
@@ -158,11 +260,22 @@ val ADDFRML_LEMM_AUT = store_thm
 
 val addEdgeToGraph_def = Define`
   addEdgeToGraph f (concrEdge pos neg sucs) g =
-    let sucIds = CAT_OPTIONS (MAP (\s. findNode (λ(n,l). l.frml = s) g) sucs)
-    in do nodeId <- findNode (λ(n,l). l.frml = f) g;
+    if sucs = []
+    then do (nodeId,nodeLabel) <- findNode (λ(n,l). l.frml = f) g;
+            newlabel <- SOME (nodeLabelAA
+                                nodeLabel.frml
+                                nodeLabel.is_final
+                                ((edgeLabelAA 0 pos neg)
+                                  :: nodeLabel.true_labels)) ;
+            updateNode nodeId newlabel g
+         od
+    else
+    let sucIds = MAP FST
+                  (CAT_OPTIONS (MAP (\s. findNode (λ(n,l). l.frml = s) g) sucs))
+    in do (nodeId,nodeLabel) <- findNode (λ(n,l). l.frml = f) g;
            oldSucPairs <- lookup nodeId g.followers ;
            oldSucs <- SOME (MAP FST oldSucPairs);
-           lstGrpId <- SOME (if oldSucs = [] then 0 else (HD oldSucs).edge_grp) ;
+           lstGrpId <- SOME (if oldSucs = [] then 1 else (HD oldSucs).edge_grp) ;
            unfolded_edges <- SOME
              (MAP (\i. (<| edge_grp := lstGrpId + 1;
                           pos_lab := pos ;
@@ -282,260 +395,593 @@ val ADDFRML_FOLDR_LEMM = store_thm
      >- metis_tac[ADDFRML_LEMM2]
   );
 
-(* val ADDEDGE_LEMM = store_thm *)
-(*   ("ADDEDGE_LEMM", *)
-(*    ``!g f e aP. wfg g ∧ MEM f (graphStates g) *)
-(*         ==> (?g2. (addEdgeToGraph f e g = SOME g2) ∧ wfg g2 *)
-(*           ∧ (g.nodeInfo = g2.nodeInfo) *)
-(*           ∧ (?i. extractTrans g2 f *)
-(*                  = extractTrans g f ∪ { (i, e.pos,e.neg,set e.sucs) }))``, *)
-(*    rpt strip_tac >> Cases_on `e` >> fs[addEdgeToGraph_def] *)
-(*    >> fs[graphStates_def,MEM_MAP] >> simp[findNode_def] *)
-(*    >> Q.HO_MATCH_ABBREV_TAC *)
-(*        `?x. (?nodeId. A nodeId ∧ ?oSP. P oSP x nodeId) ∧ Q x` *)
-(*    >> `?nodeId. A nodeId ∧ ?oSP x. P oSP x nodeId ∧ Q x` *)
-(*        suffices_by metis_tac[SWAP_EXISTS_THM] *)
-(*    >> qunabbrev_tac `P` >> qunabbrev_tac `A` >> fs[] *)
-(*    >> `?q. (FIND (λ(n,l). l.frml = (SND y).frml) (toAList g.nodeInfo) = SOME q) *)
-(*          ∧ ((λ(n,l). l.frml = (SND y).frml) q)` by ( *)
-(*        qabbrev_tac `P = (λ(n:num,l). l.frml = (SND y).frml)` *)
-(*        >> `P y` by (qunabbrev_tac `P` >> Cases_on `y` >> fs[]) *)
-(*        >> metis_tac[FIND_LEMM] *)
-(*    ) *)
-(*    >> Cases_on `q` >> rename[`_ = SOME (nId,frml)`] *)
-(*    >> qexists_tac `nId` >> rpt strip_tac *)
-(*     >- (qexists_tac `(nId,frml)` >> fs[]) *)
-(*     >- (`nId ∈ domain g.followers` by ( *)
-(*          `nId ∈ domain g.nodeInfo` suffices_by metis_tac[wfg_def] *)
-(*          >> `MEM (nId, frml) (toAList g.nodeInfo)` by metis_tac[FIND_LEMM2] *)
-(*          >> fs[MEM_toAList] >> metis_tac[domain_lookup] *)
-(*        ) *)
-(*        >> fs[domain_lookup] *)
-(*        >> Q.HO_MATCH_ABBREV_TAC *)
-(*            `?x. FOLDR addSingleEdge a_init ls = SOME x ∧ Q x` *)
-(*        >> `!lab x. MEM (lab,x) ls ==> ?h. MEM (x,h) (toAList g.nodeInfo)` by ( *)
-(*          rpt strip_tac >> qunabbrev_tac `ls` >> fs[MEM_MAP] *)
-(*          >> qabbrev_tac *)
-(*              `func = λs. *)
-(*                          OPTION_MAP FST *)
-(*                          (FIND (λ(n,l). l.frml = s) (toAList g.nodeInfo))` *)
-(*          >> `?a. MEM a l1 ∧ SOME x = func a` by metis_tac[CAT_OPTIONS_MAP_LEMM] *)
-(*          >> qunabbrev_tac `func` >> fs[] *)
-(*          >> `MEM z (toAList g.nodeInfo)` by metis_tac[FIND_LEMM2] *)
-(*          >> qexists_tac `SND z` >> fs[] *)
-(*        ) *)
-(*        >> qabbrev_tac `LABEL = *)
-(*             <|edge_grp := (if v = [] then 0 else (HD (MAP FST v)).edge_grp) + 1; *)
-(*               pos_lab := l; *)
-(*               neg_lab := l0|>` *)
-(*        >> qabbrev_tac ` *)
-(*             TO_LABELS = λl. *)
-(*                 MAP (λi. (LABEL,i)) *)
-(*                 (CAT_OPTIONS *)
-(*                    (MAP *)
-(*                     (λs. *)
-(*                      OPTION_MAP FST *)
-(*                      (FIND (λ(n,l). l.frml = s) (toAList g.nodeInfo))) l))` *)
-(*        >> `ls = TO_LABELS l1` by (qunabbrev_tac `TO_LABELS` >> simp[]) *)
-(*        >> `!qs fs. ((!lab x. MEM (lab,x) qs *)
-(*                           ==> (?h. MEM (x,h) (toAList g.nodeInfo) *)
-(*                                 ∧ (lab = LABEL))) *)
-(*                   ∧ (qs = TO_LABELS fs)) *)
-(*              ==> ?m. (FOLDR addSingleEdge a_init qs = SOME m) *)
-(*                    ∧ (g.nodeInfo = m.nodeInfo) *)
-(*                    ∧ (wfg m) *)
-(*                    ∧ (?e. ((LABEL.edge_grp,l,l0,e) ∈ extractTrans m frml.frml) *)
-(*                          ∧ (!x. MEM (LABEL, x) qs *)
-(*                              ==> ?node. (lookup x m.nodeInfo = SOME node) *)
-(*                                       ∧ (node.frml ∈ e))) *)
-(*                    ∧ (?i. extractTrans m frml.frml *)
-(*                             = extractTrans g frml.frml ∪ {(i,l,l0,set fs)})` by ( *)
-(*            Induct_on `qs` >> fs[] *)
-(*             >- (qunabbrev_tac `a_init` >> simp[extractTrans_def] >> rpt strip_tac *)
-(*                 >- (qexists_tac `LABEL` >> qunabbrev_tac `LABEL` >> fs[]) *)
-(*                 >- () *)
-(*                ) *)
-(*             >- (rpt strip_tac *)
-(*                 >> `∀lab x. MEM (lab,x) qs *)
-(*                       ⇒ (∃h. MEM (x,h) (toAList g.nodeInfo) ∧ (lab = LABEL))` *)
-(*                     by metis_tac[] *)
-(*                 >> `∃m. (FOLDR addSingleEdge a_init qs = SOME m) *)
-(*                       ∧ (g.nodeInfo = m.nodeInfo) *)
-(*                       ∧ (wfg m) *)
-(*                       ∧ (∃e. *)
-(*                           (LABEL.edge_grp,l,l0,e) ∈ extractTrans m frml.frml *)
-(*                           ∧ ∀x. *)
-(*                            MEM (LABEL,x) qs ⇒ *)
-(*                            ∃node. lookup x m.nodeInfo = SOME node *)
-(*                                 ∧ node.frml ∈ e)` *)
-(*                      by metis_tac[] *)
-(*                 >> `?m2. (addSingleEdge h (SOME m) = SOME m2) *)
-(*                        ∧ (g.nodeInfo = m2.nodeInfo) *)
-(*                        ∧ (wfg m2) *)
-(*                        ∧ (∃e. (LABEL.edge_grp,l,l0,e) *)
-(*                                 ∈ extractTrans m2 (SND y).frml *)
-(*                              ∧ ∀x. *)
-(*                                (LABEL,x) = h ∨ MEM (LABEL,x) qs ⇒ *)
-(*                                  ∃node. lookup x m2.nodeInfo = SOME node *)
-(*                                       ∧ node.frml ∈ e)` *)
-(*                      suffices_by fs[] *)
-(*                 >> qunabbrev_tac `addSingleEdge` >> Cases_on `h` *)
-(*                 >> simp[] *)
-(*                 >> `?nG. addEdge nId (q,r) m = SOME nG` by ( *)
-(*                      simp[addEdge_def] *)
-(*                      >> Q.HO_MATCH_ABBREV_TAC `?nG. P ∧ A nG` *)
-(*                      >> `P ∧ (P ==> ?nG. A nG)` suffices_by fs[] *)
-(*                      >> qunabbrev_tac `P` >> qunabbrev_tac `A` *)
-(*                      >> rpt strip_tac *)
-(*                       >- (`MEM (nId,frml) (toAList g.nodeInfo)` *)
-(*                              by metis_tac[FIND_LEMM2] *)
-(*                           >> fs[MEM_toAList,domain_lookup] *)
-(*                           >> metis_tac[] *)
-(*                          ) *)
-(*                       >- (`∃h. MEM (r,h) (toAList g.nodeInfo)` by metis_tac[] *)
-(*                           >> fs[MEM_toAList,domain_lookup] *)
-(*                           >> metis_tac[] *)
-(*                          ) *)
-(*                       >- (`nId ∈ domain m.followers` by metis_tac[wfg_def] *)
-(*                           >> `?fol_o. lookup nId m.followers = SOME fol_o` *)
-(*                              by metis_tac[domain_lookup] *)
-(*                           >> fs[] *)
-(*                          ) *)
-(*                  ) *)
-(*                 >> qexists_tac `nG` >> simp[] *)
-(*                 >> `wfg nG` by metis_tac[addEdge_preserves_wfg] *)
-(*                 >> POP_ASSUM mp_tac >> POP_ASSUM mp_tac *)
-(*                 >> simp[addEdge_def] >> rpt strip_tac *)
-(*                 >> Cases_on `m` >> fs[gfg_fn_updates] *)
-(*                 >> fs[gfg_component_equality] *)
-(*                 >> `?node. lookup r nG.nodeInfo = SOME node` *)
-(*                    by metis_tac[domain_lookup] *)
-(*                 >> qexists_tac `e ∪ {node.frml}` *)
-(*                 >> rpt strip_tac *)
-(*                 >- (fs[extractTrans_def] *)
-(*                     >> qexists_tac `LABEL` >> simp[SET_EQ_SUBSET,SUBSET_DEF] *)
-(*                     >> rpt strip_tac *)
-(*                     >- (qunabbrev_tac `LABEL` >> fs[]) *)
-(*                     >- (qunabbrev_tac `LABEL` >> fs[]) *)
-(*                     >- ( *)
-(*                      qexists_tac `suc` >> simp[] >> qexists_tac `sucId` *)
-(*                      >> simp[] *)
-(*                      >> Q.HO_MATCH_ABBREV_TAC ` *)
-(*                          MEM (LABEL,sucId) (OPTION_TO_LIST M_L)` *)
-(*                      >> qabbrev_tac `M_L0 = *)
-(*                          do node <- *)
-(*                               findNode (λ(n',l). l.frml = (SND y).frml) *)
-(*                                        (gfg nG.nodeInfo s0 nG.preds nG.next); *)
-(*                             lookup node s0 *)
-(*                          od` *)
-(*                      >> `IS_SOME M_L0` *)
-(*                            by metis_tac[MEM,OPTION_TO_LIST_def, *)
-(*                                         NOT_IS_SOME_EQ_NONE] *)
-(*                      >> `IS_SOME M_L` by ( *)
-(*                          qunabbrev_tac `M_L` >> POP_ASSUM mp_tac *)
-(*                          >> qunabbrev_tac `M_L0` >> simp[IS_SOME_EXISTS] *)
-(*                          >> rpt strip_tac >> Cases_on `node' = nId` *)
-(*                          >- (qexists_tac `((q,r)::followers_old)` *)
-(*                              >> qexists_tac `nId` >> fs[findNode_def] *)
-(*                              >> metis_tac[lookup_insert] *)
-(*                             ) *)
-(*                          >- (qexists_tac `x'` >> qexists_tac `node'` *)
-(*                              >> fs[findNode_def] >> metis_tac[lookup_insert] *)
-(*                             ) *)
-(*                      ) *)
-(*                      >> fs[IS_SOME_EXISTS,OPTION_TO_LIST_def] *)
-(*                      >> `MEM (label',sucId) x'` by metis_tac[OPTION_TO_LIST_def] *)
-(*                      >> qunabbrev_tac `M_L` >> qunabbrev_tac `M_L0` >> fs[] *)
-(*                      >> `node' = node''` by ( *)
-(*                           Cases_on `nG` >> fs[findNode_def] *)
-(*                           >> rw[] >> metis_tac[SOME_11] *)
-(*                      ) *)
-(*                      >> `LABEL = label'` by ( *)
-(*                          qunabbrev_tac `LABEL` *)
-(*                          >> fs[theorem "edgeLabelAA_component_equality"] *)
-(*                      ) *)
-(*                      >> rw[] >> Cases_on `node' = nId` >> fs[] *)
-(*                      >- (rw[] *)
-(*                          >> `x'' = (q,r)::followers_old` *)
-(*                             by metis_tac[lookup_insert,SOME_11] *)
-(*                          >> metis_tac[MEM] *)
-(*                         ) *)
-(*                      >- (rw[] >> metis_tac[lookup_insert,SOME_11]) *)
-(*                      ) *)
-(*                     >- (rw[] >> qexists_tac `node` >> simp[] >> qexists_tac `r` *)
-(*                         >> simp[] *)
-(*                         >> Q.HO_MATCH_ABBREV_TAC ` *)
-(*                             MEM (LABEL,r) (OPTION_TO_LIST M_L)` *)
-(*                         >> `IS_SOME M_L` by ( *)
-(*                             simp[IS_SOME_EXISTS] >> qunabbrev_tac `M_L` *)
-(*                             >> qexists_tac `(q,r)::followers_old` >> fs[] *)
-(*                             >> qexists_tac `nId` >> fs[findNode_def] *)
-(*                             >> rpt strip_tac >>  metis_tac[lookup_insert] *)
-(*                          ) *)
-(*                         >> fs[IS_SOME_EXISTS] *)
-(*                         >> `MEM (LABEL,r) x` suffices_by *)
-(*                               metis_tac[OPTION_TO_LIST_def,NOT_IS_SOME_EQ_NONE] *)
-(*                         >> qunabbrev_tac `M_L` >> fs[findNode_def] *)
-(*                         >> `node' = nId` by fs[] >> rw[] *)
-(*                         >> `q = LABEL` by metis_tac[] >> rw[] *)
-(*                         >> metis_tac[lookup_insert,SOME_11,MEM] *)
-(*                        ) *)
-(*                     >- (Cases_on `x = node.frml` >> fs[] *)
-(*                         >> `LABEL = label'` by ( *)
-(*                              qunabbrev_tac `LABEL` *)
-(*                              >> fs[theorem "edgeLabelAA_component_equality"] *)
-(*                          ) *)
-(*                         >> rw[] >> qexists_tac `suc` >> fs[] *)
-(*                         >> qexists_tac `sucId` >> fs[] *)
-(*                         >> Q.HO_MATCH_ABBREV_TAC ` *)
-(*                               MEM (LABEL,sucId) (OPTION_TO_LIST M_0)` *)
-(*                         >> qabbrev_tac ` *)
-(*                             M_L =  do *)
-(*                                      node <- findNode *)
-(*                                               (λ(n,l). l.frml = (SND y).frml) *)
-(*                                               nG; *)
-(*                                      lookup node nG.followers *)
-(*                                     od` *)
-(*                         >> `IS_SOME M_L` *)
-(*                               by metis_tac[MEM,OPTION_TO_LIST_def, *)
-(*                                            NOT_IS_SOME_EQ_NONE] *)
-(*                         >> `IS_SOME M_0` by ( *)
-(*                              qunabbrev_tac `M_L` >> POP_ASSUM mp_tac *)
-(*                              >> qunabbrev_tac `M_0` >> simp[IS_SOME_EXISTS] *)
-(*                              >> rpt strip_tac >> Cases_on `node' = nId` *)
-(*                              >- (qexists_tac `followers_old` *)
-(*                                  >> qexists_tac `nId` >> fs[findNode_def] *)
-(*                                 ) *)
-(*                              >- (qexists_tac `x` >> qexists_tac `node'` *)
-(*                                  >> fs[findNode_def] >> metis_tac[lookup_insert] *)
-(*                                 ) *)
-(*                          ) *)
-(*                         >> fs[IS_SOME_EXISTS,OPTION_TO_LIST_def] *)
-(*                         >> `MEM (LABEL,sucId) x` by metis_tac[OPTION_TO_LIST_def] *)
-(*                         >> qunabbrev_tac `M_L` >> qunabbrev_tac `M_0` >> fs[] *)
-(*                         >> `node' = node''` by ( *)
-(*                              Cases_on `nG` >> fs[findNode_def] *)
-(*                              >> rw[] >> metis_tac[SOME_11] *)
-(*                          ) *)
-(*                         >> rw[] *)
-(*                         >> Cases_on `node' = nId` >> fs[] *)
-(*                         >- (rw[] *)
-(*                             >> `x = (q,r)::followers_old` by metis_tac[lookup_insert,SOME_11] *)
-(*                             >> `~(sucId = r)` by ( *)
-(*                                 `~(node = suc)` suffices_by metis_tac[SOME_11] *)
-(*                                 >> fs[theorem "nodeLabelAA_component_equality"] *)
-(*                              ) *)
-(*                             >> `~((LABEL,sucId) = (q,r))` by fs[] *)
-(*                             >> metis_tac[MEM] *)
-(*                            ) *)
-(*                         >- (rw[] >> metis_tac[lookup_insert,SOME_11]) *)
-(*                        ) *)
-(*                    ) *)
-(*                     >- fs[] *)
-(*                     >- (fs[] >> metis_tac[]) *)
-(*                    ) *)
-(*                ) *)
-(*        >> `!qs.  *)
+val ADD_0EDGE_LEMM = store_thm
+  ("ADD_0EDGE_LEMM",
+   ``!g g2 nId lab edge.
+        let NEW_LAB =
+              nodeLabelAA lab.frml lab.is_final (edge::lab.true_labels)
+        in
+        (lookup nId g.nodeInfo = SOME lab)
+        ∧ unique_node_formula g
+        ∧ (updateNode nId NEW_LAB g = SOME g2)
+        ==> unique_node_formula g2``,
+   fs[unique_node_formula_def,updateNode_def,graphStatesWithId_def]
+   >> rpt strip_tac >> fs[MEM_MAP]
+   >> first_x_assum (qspec_then `id` mp_tac) >> rpt strip_tac
+   >> qabbrev_tac `nodeInfo2 =
+                    insert nId
+                     (nodeLabelAA lab.frml lab.is_final
+                      (edge::lab.true_labels)) g.nodeInfo`
+   >> Cases_on `y` >> Cases_on `y'` >> fs[] >> rw[]
+   >> first_x_assum (qspec_then `r.frml` mp_tac) >> simp[] >> rpt strip_tac
+   >> `(lookup id nodeInfo2 = SOME r) ∧ (lookup oId nodeInfo2 = SOME r')`
+      by metis_tac[MEM_toAList]
+   >> `?z1. (lookup id g.nodeInfo = SOME z1) ∧ (z1.frml = r.frml)` by (
+       qunabbrev_tac `nodeInfo2` >> Cases_on `id = nId`
+       >> fs[lookup_insert] >> Cases_on `r` >> fs[]
+   )
+   >> `?z2. (lookup oId g.nodeInfo = SOME z2) ∧ (z2.frml = r.frml)` by (
+       qunabbrev_tac `nodeInfo2` >> Cases_on `oId = nId`
+       >> fs[lookup_insert] >> Cases_on `r'` >> fs[]
+   )
+   >> `∃y.
+         (id,r.frml) = (λ(id,label). (id,label.frml)) y
+        ∧ MEM y (toAList g.nodeInfo)` by (
+       qexists_tac `(id,z1)` >> fs[MEM_toAList]
+   )
+   >> `∀oId'.
+        (∃y.
+          (oId',r.frml) = (λ(id,label). (id,label.frml)) y
+        ∧ MEM y (toAList g.nodeInfo)) ⇒ (id = oId')` by metis_tac[]
+   >> first_x_assum (qspec_then `oId` mp_tac) >> simp[]
+   >> `∃y.
+        (oId,r.frml) = (λ(id,label). (id,label.frml)) y
+        ∧ MEM y (toAList g.nodeInfo)` by (
+       qexists_tac `(oId,z2)` >> fs[MEM_toAList]
+   ) >> metis_tac[]
+  );
+
+val ADDEDGE_LEMM = store_thm
+  ("ADDEDGE_LEMM",
+   ``!g f e aP. wfg g ∧ MEM f (graphStates g)
+            ∧ unique_node_formula g
+        ==> (?g2. (addEdgeToGraph f e g = SOME g2) ∧ wfg g2
+          ∧ (set (graphStatesWithId g) = set (graphStatesWithId g2))
+          ∧ (unique_node_formula g2)
+          ∧ (!h.
+                 if h = f
+                 then ?i. extractTrans g2 h
+                        = extractTrans g h ∪ { (i, e.pos,e.neg,set e.sucs) }
+                 else extractTrans g2 h = extractTrans g h))``,
+   rpt strip_tac >> Cases_on `e` >> fs[addEdgeToGraph_def]
+   >> fs[graphStates_def,MEM_MAP] (* >> simp[findNode_def] *)
+   >> Cases_on `l1` >> fs[] >> rpt strip_tac
+   >> `?q. (findNode (λ(n,l). l.frml = (SND y).frml) g = SOME q)
+        ∧ ((λ(n,l). l.frml = (SND y).frml) q)` by (
+       simp[findNode_def]
+       >> qabbrev_tac `P = (λ(n:num,l). l.frml = (SND y).frml)`
+       >> `P y` by (qunabbrev_tac `P` >> Cases_on `y` >> fs[])
+       >> metis_tac[FIND_LEMM]
+   )
+   >- (
+     Q.HO_MATCH_ABBREV_TAC
+       `?g2. (?nodeId. A nodeId ∧ P g2 nodeId) ∧ Q g2`
+     >> `?nodeId. A nodeId ∧ ?g2. P g2 nodeId ∧ Q g2` suffices_by metis_tac[]
+     >> qunabbrev_tac `A` >> qunabbrev_tac `P` >> fs[]
+     >> Cases_on `q` >> fs[] >> rename[`_ = SOME (nId,frml)`]
+     >> Q.HO_MATCH_ABBREV_TAC
+         `?g2. updateNode nId NEW_LAB g = SOME g2 ∧ Q g2`
+     >> `∃x. updateNode nId NEW_LAB g = SOME x` by (
+         simp[updateNode_def] >> fs[findNode_def]
+         >> `MEM (nId, frml) (toAList g.nodeInfo)` by metis_tac[FIND_LEMM2]
+         >> fs[MEM_toAList] >> metis_tac[domain_lookup]
+     )
+     >> `g.followers = x.followers`
+        by fs[updateNode_def,gfg_component_equality]
+     >> qexists_tac `x` >> qunabbrev_tac `Q` >> simp[]
+     >> Q.HO_MATCH_ABBREV_TAC `A ∧ B ∧ C`
+     >> `A ∧ B ∧ (A ∧ B ==> C)` suffices_by metis_tac[]
+     >> qunabbrev_tac `A` >> qunabbrev_tac `B` >> qunabbrev_tac `C`
+     >> `lookup nId g.nodeInfo = SOME frml` by (
+         fs[unique_node_formula_def,graphStatesWithId_def,findNode_def]
+         >> `MEM (nId,frml) (toAList g.nodeInfo)
+           ∧ (λ(n,l). l.frml = (SND y).frml) (nId,frml)`
+            by metis_tac[FIND_LEMM2]
+         >> metis_tac[MEM_toAList]
+     )
+     >> `unique_node_formula x` by metis_tac[ADD_0EDGE_LEMM]
+     (* >> `!n. OPTION_MAP (λ(id,lab). (id,lab.frml)) *)
+     (*           (findNode (λ(n,l). l.frml = (SND y).frml) g) *)
+     (*          = OPTION_MAP (λ(id,lab). (id,lab.frml)) *)
+     (*            (findNode (λ(n,l). l.frml = (SND y).frml) x)` by ( *)
+     (*     rpt strip_tac *)
+     (*     >> `(OPTION_MAP (λ(id,lab). (id,lab.frml)) *)
+     (*          (findNode (λ(n,l). l.frml = (SND y).frml) x)) *)
+     (*         = (SOME (nId,f))` suffices_by fs[] *)
+     (*     >> `findNode (λ(n,l). l.frml = (SND y).frml) x = SOME (nId,NEW_LAB)` *)
+     (*        suffices_by (qunabbrev_tac `NEW_LAB` >> fs[]) *)
+     (*     >> fs[findNode_def,updateNode_def] >> rw[] *)
+     (*     >> qabbrev_tac `nodeList2 = insert nId NEW_LAB g.nodeInfo` *)
+     (*     >> `?id l. MEM (id,l) (toAList nodeList2) *)
+     (*              ∧ (λ(n,l). l.frml = (SND y).frml) (id,l)` by ( *)
+     (*         fs[MEM_toAList] >> qunabbrev_tac `nodeList2` *)
+     (*         >> fs[lookup_insert] >> qexists_tac `nId` >> fs[] *)
+     (*         >> qunabbrev_tac `NEW_LAB` >> fs[] *)
+     (*     ) *)
+     (*     >> `?k. FIND (λ(n,l). l.frml = (SND y).frml) *)
+     (*              (toAList nodeList2) = SOME k` by metis_tac[FIND_LEMM] *)
+     (*     >> fs[unique_node_formula_def,graphStatesWithId_def] *)
+     (*     >> Cases_on `k` *)
+     (*     >> first_x_assum (qspec_then `q` mp_tac) >> rpt strip_tac *)
+     (*     >> first_x_assum (qspec_then `r.frml` mp_tac) >> rpt strip_tac *)
+     (*     >> `MEM (q,r.frml) *)
+     (*          (MAP (λ(id,label). (id,label.frml)) (toAList nodeList2))` by ( *)
+     (*         simp[MEM_MAP] >> qexists_tac `(q,r)` >> fs[] *)
+     (*         >> metis_tac[FIND_LEMM2] *)
+     (*     ) *)
+     (*     >> `∀oId. *)
+     (*          MEM (oId,r.frml) *)
+     (*          (MAP (λ(id,label). (id,label.frml)) (toAList nodeList2)) ⇒ *)
+     (*          q = oId` by metis_tac[] *)
+     (*     >> first_x_assum (qspec_then `nId` mp_tac) >> rpt strip_tac *)
+     (*     >> `MEM (nId,r) *)
+     (* ) *)
+     >> rpt strip_tac
+      >- metis_tac[updateNode_preserves_wfg]
+      >- (simp[graphStatesWithId_def,SET_EQ_SUBSET,SUBSET_DEF] >> rpt strip_tac
+          >> fs[MEM_MAP,updateNode_def] >> Cases_on `x'` >> Cases_on `y'`
+          >> Cases_on `q = nId` >> fs[findNode_def] >> rw[]
+           >- (qexists_tac `(nId, NEW_LAB)` >> qunabbrev_tac `NEW_LAB` >> fs[]
+               >> qabbrev_tac `P = (λ(n:num,l). l.frml = (SND y).frml)`
+               >> `P (nId,frml) ∧ MEM (nId,frml) (toAList g.nodeInfo)`
+                   by metis_tac[FIND_LEMM2]
+               >> qunabbrev_tac `P` >> fs[]
+               >> `lookup nId g.nodeInfo = SOME r'` by metis_tac[MEM_toAList]
+               >> `lookup nId g.nodeInfo = SOME frml` by metis_tac[MEM_toAList]
+               >> `r' = frml` by metis_tac[SOME_11] >> rw[]
+               >> rw[MEM_toAList] >> fs[gfg_component_equality] >> rw[]
+               >> metis_tac[lookup_insert]
+              )
+           >- (qexists_tac `(q,r')` >> fs[MEM_toAList,gfg_component_equality]
+               >> rw[]  >> metis_tac[lookup_insert])
+           >- (qexists_tac `(nId,frml)` >> (* qunabbrev_tac `NEW_LAB` >> *) fs[]
+               >> qabbrev_tac `P = (λ(n:num,l). l.frml = (SND y).frml)`
+               >> `P (nId,frml) ∧ MEM (nId,frml) (toAList g.nodeInfo)`
+                  by metis_tac[FIND_LEMM2]
+               >> qunabbrev_tac `P` >> fs[]
+               >> `lookup nId g.nodeInfo = SOME frml` by metis_tac[MEM_toAList]
+               >> fs[gfg_component_equality]
+               >> `lookup nId (insert nId NEW_LAB g.nodeInfo) = SOME r'`
+                     by metis_tac[MEM_toAList]
+               >> fs[lookup_insert] >> qunabbrev_tac `r'` >> fs[]
+              )
+           >- (qexists_tac `(q,r')` >> fs[MEM_toAList,gfg_component_equality]
+              >> metis_tac[lookup_insert])
+         )
+      >- fs[]
+      >- (Cases_on `h = f` >> fs[]
+          >- (qexists_tac `0` >> simp[SET_EQ_SUBSET,SUBSET_DEF] >> rpt strip_tac
+            >> fs[extractTrans_def]
+            >- (
+             qexists_tac `label` >> fs[]
+             >> simp[SET_EQ_SUBSET,SUBSET_DEF] >> rpt strip_tac
+             >- (
+              fs[OPTION_TO_LIST_MEM]
+              >> rename[`findNode _ x = SOME x1`]
+              >> `SOME ((λ(id,label). (id,label.frml)) x1)
+                   = FIND (λa. SND a = (SND y).frml) (graphStatesWithId x)`
+                 by metis_tac[OPTION_MAP_DEF,UNIQUE_NODE_FORM_LEMM]
+              >> Cases_on `x1` >> fs[]
+              >> `MEM (q,r.frml) (graphStatesWithId x)
+                  ∧ ((λa. SND a = (SND y).frml) (q,r.frml))`
+                 by (Q.HO_MATCH_ABBREV_TAC `MEM A L ∧ P A`
+                     >> metis_tac[FIND_LEMM2])
+              >> `MEM (q,r.frml) (graphStatesWithId g)` by metis_tac[MEM]
+              >> `MEM (nId,frml.frml) (graphStatesWithId g)` by (
+                  PURE_REWRITE_TAC[graphStatesWithId_def,MEM_MAP]
+                  >> qexists_tac `(nId,frml)` >> fs[]
+                  >> metis_tac[MEM_toAList]
+              )
+              >> `q = nId` by (
+                  `SND (q,r.frml) = f` by fs[]
+                  >> `SND (nId,r.frml) = f` by fs[]
+                  >> IMP_RES_TAC UNIQUE_NODE_FORM_LEMM2 >> fs[]
+              )
+              >> rw[]
+              >> Cases_on `sucId = nId` >> fs[] >> rw[]
+              >- (qexists_tac `frml` >> fs[]
+                  >> `MEM (nId,suc) (toAList x.nodeInfo)`
+                      by metis_tac[MEM_toAList]
+                  >> `MEM (nId,suc.frml) (graphStatesWithId x)` by (
+                        simp[graphStatesWithId_def,MEM_MAP]
+                        >> qexists_tac `(nId,suc)` >> fs[]
+                    )
+                  >> `MEM (nId,suc.frml) (graphStatesWithId g)` by fs[]
+                  >> `suc.frml = frml.frml` by (
+                        fs[graphStatesWithId_def,MEM_MAP]
+                        >> rename[`(nId,suc.frml) = _ y1`]
+                        >> POP_ASSUM mp_tac >> POP_ASSUM mp_tac
+                        >> POP_ASSUM mp_tac >> POP_ASSUM mp_tac
+                        >> rename[`(nId,suc.frml) = _ y2`] >> rpt strip_tac
+                        >> Cases_on `y1` >> Cases_on `y2` >> fs[] >> rw[]
+                        >> metis_tac[MEM_toAList,SOME_11]
+                    )
+                  >> rw[] >> qexists_tac `nId` >> fs[]
+                  >> metis_tac[]
+                 )
+              >- (
+               qexists_tac `suc` >> fs[] >> qexists_tac `sucId`
+               >> `∃l. lookup nId g.followers = SOME l ∧ MEM (label,sucId) l`
+                  by metis_tac[]
+               >> rpt strip_tac >> fs[updateNode_def] >> Cases_on `g`
+               >> fs[gfg_component_equality] >> metis_tac[lookup_insert]
+              )
+             )
+             >- (fs[OPTION_TO_LIST_MEM] >> Cases_on `sucId = nId` >> fs[]
+                 >> rw[]
+              >- (
+               `suc = frml` by metis_tac[SOME_11]
+               >> qexists_tac `NEW_LAB` >> fs[] >> rpt strip_tac
+               >- (qunabbrev_tac `NEW_LAB` >> fs[])
+               >- (qexists_tac `nId` >> fs[]
+                   >> `lookup nId x.nodeInfo = SOME NEW_LAB` by (
+                        fs[updateNode_def,gfg_component_equality]
+                        >> metis_tac[lookup_insert]
+                    ) >> fs[]
+                   >> qexists_tac `l'` >> fs[] >> qexists_tac `(nId,NEW_LAB)`
+                   >> fs[] >> rpt strip_tac
+                   >> simp[findNode_def]
+                   >> `MEM (nId, NEW_LAB) (toAList x.nodeInfo)`
+                      by metis_tac[MEM_toAList]
+                   >> `(λ(n,l). l.frml = (SND y).frml) (nId,NEW_LAB)` by (
+                        qunabbrev_tac `NEW_LAB` >> fs[]
+                    )
+                   >> `?z. FIND (λ(n,l). l.frml = (SND y).frml)
+                                  (toAList x.nodeInfo) = SOME z`
+                      by metis_tac[FIND_LEMM]
+                   >> `MEM z (toAList x.nodeInfo)
+                    ∧ (λ(n,l). l.frml = (SND y).frml) z`
+                      by metis_tac[FIND_LEMM2]
+                   >> Cases_on `z`
+                   >> `MEM (q,r.frml) (graphStatesWithId g)`
+                      by (fs[MEM_MAP,graphStatesWithId_def]
+                          >> qexists_tac `(q,r)` >> fs[]
+                         )
+                   >> `MEM (nId,NEW_LAB.frml) (graphStatesWithId g)`
+                      by (fs[MEM_MAP,graphStatesWithId_def]
+                          >> qexists_tac `(nId,NEW_LAB)` >> fs[]
+                         )
+                   >> `NEW_LAB.frml = r.frml`
+                        by (qunabbrev_tac `NEW_LAB` >> fs[])
+                   >> IMP_RES_TAC UNIQUE_NODE_FORM_LEMM2 >> fs[]
+                   >> first_x_assum (qspec_then `(nId,r.frml)` mp_tac)
+                   >> simp[] >> rpt strip_tac >> rw[]
+                   >> metis_tac[MEM_toAList,SOME_11]
+                  )
+                  )
+              >- (
+
+                  )
+
+)
+
+)
+)
+)
+
+               )
+            >- (
+             
+
+)
+
+               >> qexists_tac `suc` >> fs[] >> qexists_tac `sucId` >> fs[]
+               >> `q' = nId` suffices_by (
+                    rpt strip_tac >> rw[] >> fs[]
+)
+
+
+)
+
+
+            `MEM (sucId,suc) (toAList x.nodeInfo)`
+               by metis_tac[MEM_toAList]
+             >> qabbrev_tac `h = (λ(id:num,label). (id,label.frml))`
+             >> `MEM (h (sucId,suc)) (MAP h (toAList g.nodeInfo))`
+               by metis_tac[MEM_MAP,MEM]
+             >> fs[MEM_MAP] >> Cases_on `y'` >> qunabbrev_tac `h` >> fs[]
+             >> qexists_tac `r` >> fs[] >> qexists_tac `q`
+             >> qabbrev_tac `L = λg:(α nodeLabelAA, α edgeLabelAA) gfg.
+                                  do
+                                  (nId,nodeLabel)
+                                      <- findNode (λ(n,l). l.frml
+                                                   = (SND y).frml) g;
+                                  lookup nId g.followers
+                                  od`
+              >> `(MEM (label,q) (OPTION_TO_LIST (L g)))
+                ∧ (SOME r = (lookup q g.nodeInfo))` suffices_by fs[]
+              >> `MEM (label,q) (OPTION_TO_LIST (L x))` by fs[]
+              >> Cases_on `L x`
+              >- metis_tac[OPTION_TO_LIST_def,MEM]
+              >- (
+               rename[`L x = SOME l_x`]
+               >> `MEM (label,q) l_x` by fs[OPTION_TO_LIST_def]
+               >> Cases_on `L g` >> qunabbrev_tac `L` >> fs[findNode_def]
+               >- fs[findNode_def]
+               >- (`x.followers = g.followers`
+                       by metis_tac[updateNode_preserves_edges]
+                   >> rename[`_ (toAList g.nodeInfo) = SOME n2`]
+                   >> rename[`_ n1 = SOME l_x`,`FIND _ _ = SOME n1`]
+                   >> `~((λ(nId,nodeLabel). lookup nId g.followers) n2 = NONE)`
+                      suffices_by fs[]
+                   >> rw[] >> fs[updateNode_def]
+                   >> `MEM n2 (toAList g.nodeInfo)` by metis_tac[FIND_LEMM2]
+                   >> fs[wfg_def] >> Cases_on `n2` >> fs[]
+                   >> `~(q' ∈ domain g.followers)` by fs[domain_lookup]
+                   >> metis_tac[MEM_toAList,domain_lookup]
+                  )
+               >- (fs[OPTION_TO_LIST_def] >> rw[]
+                   >- (rename[`_ (nId,frml) = SOME x1`]
+                       >> fs[]
+                       >> rename[`(λ(nId,nodeLabel). lookup nId x.followers) x2
+                                           = SOME l_x`]
+                       >> Cases_on `x2`
+             >> `q = q'` by (
+                 `(FIND (λ(n,l). l.frml = (SND y).frml) (toAList x.nodeInfo))
+                 = (FIND (λ(n,l). l.frml = (SND y).frml) (toAList g.nodeInfo))`
+                 by (fs[updateNode_def,FIND_def] >> rw[] >> fs[]
+                     >> Induct_on `g.nodeInfo` >> fs[]
+                     >- rw[] >> fs[insert_def]
+
+)
+)
+
+)
+)
+)
+)
+
+)
+
+   >> Q.HO_MATCH_ABBREV_TAC
+       `?x. (?nodeId. A nodeId ∧ P x nodeId) ∧ Q x`
+   (* >> Q.HO_MATCH_ABBREV_TAC *)
+   (*     `?x. (?nodeId. A nodeId ∧ ?oSP. P oSP x nodeId) ∧ Q x` *)
+   >> `?nodeId. A nodeId ∧ ?x. P x nodeId ∧ Q x`
+       suffices_by metis_tac[SWAP_EXISTS_THM]
+   >> qunabbrev_tac `P` >> qunabbrev_tac `A` >> fs[]
+   >> Cases_on `q` >> fs[] >> rename[`_ = SOME (nId,frml)`]
+   (* >> qexists_tac `nId` >> rpt strip_tac *)
+   (*  >- (qexists_tac `(nId,frml)` >> fs[]) *)
+    >- (`nId ∈ domain g.followers` by (
+         `nId ∈ domain g.nodeInfo` suffices_by metis_tac[wfg_def]
+         >> `MEM (nId, frml) (toAList g.nodeInfo)` by metis_tac[FIND_LEMM2]
+         >> fs[MEM_toAList] >> metis_tac[domain_lookup]
+       )
+       >> fs[domain_lookup]
+       >> Q.HO_MATCH_ABBREV_TAC
+           `?x. FOLDR addSingleEdge a_init ls = SOME x ∧ Q x`
+       >> `!lab x. MEM (lab,x) ls ==> ?h. MEM (x,h) (toAList g.nodeInfo)` by (
+         rpt strip_tac >> qunabbrev_tac `ls` >> fs[MEM_MAP]
+         >> qabbrev_tac
+             `func = λs. (FIND (λ(n,l). l.frml = s) (toAList g.nodeInfo))`
+         >> `?a. MEM a l1 ∧ SOME y' = func a` by metis_tac[CAT_OPTIONS_MAP_LEMM]
+         >> qunabbrev_tac `func` >> fs[]
+         >> `MEM y' (toAList g.nodeInfo)` by metis_tac[FIND_LEMM2]
+         >> qexists_tac `SND y'` >> fs[]
+       )
+       >> qabbrev_tac `LABEL =
+            <|edge_grp := (if v = [] then 1 else (HD (MAP FST v)).edge_grp) + 1;
+              pos_lab := l;
+              neg_lab := l0|>`
+       >> qabbrev_tac `
+            TO_LABELS = λl.
+                MAP (λi. (LABEL,i))
+                (MAP FST
+                 (CAT_OPTIONS
+                   (MAP
+                    (λs.
+                     (FIND (λ(n,l). l.frml = s) (toAList g.nodeInfo))) l)))`
+       >> `ls = TO_LABELS l1` by (qunabbrev_tac `TO_LABELS` >> simp[])
+       >> `!qs fs. ((!lab x. MEM (lab,x) qs
+                          ==> (?h. MEM (x,h) (toAList g.nodeInfo)
+                                ∧ (lab = LABEL)))
+                  ∧ (qs = TO_LABELS fs))
+             ==> ?m. (FOLDR addSingleEdge a_init qs = SOME m)
+                   ∧ (g.nodeInfo = m.nodeInfo)
+                   ∧ (wfg m)
+                   (* ∧ (?e. ((LABEL.edge_grp,l,l0,e) ∈ extractTrans m frml.frml) *)
+                   (*       ∧ (!x. MEM (LABEL, x) qs *)
+                   (*           ==> ?node. (lookup x m.nodeInfo = SOME node) *)
+                   (*                    ∧ (node.frml ∈ e))) *)
+                   ∧ (?i. extractTrans m frml.frml
+                            = extractTrans g frml.frml ∪ {(i,l,l0,set fs)})` by (
+           Induct_on `qs` >> fs[]
+            >- (qunabbrev_tac `a_init` >> simp[extractTrans_def] >> rpt strip_tac
+                >- (qexists_tac `LABEL` >> qunabbrev_tac `LABEL` >> fs[])
+                >- ()
+               )
+            >- (rpt strip_tac
+                >> `∀lab x. MEM (lab,x) qs
+                      ⇒ (∃h. MEM (x,h) (toAList g.nodeInfo) ∧ (lab = LABEL))`
+                    by metis_tac[]
+                >> `∃m. (FOLDR addSingleEdge a_init qs = SOME m)
+                      ∧ (g.nodeInfo = m.nodeInfo)
+                      ∧ (wfg m)
+                      ∧ (∃e.
+                          (LABEL.edge_grp,l,l0,e) ∈ extractTrans m frml.frml
+                          ∧ ∀x.
+                           MEM (LABEL,x) qs ⇒
+                           ∃node. lookup x m.nodeInfo = SOME node
+                                ∧ node.frml ∈ e)`
+                     by metis_tac[]
+                >> `?m2. (addSingleEdge h (SOME m) = SOME m2)
+                       ∧ (g.nodeInfo = m2.nodeInfo)
+                       ∧ (wfg m2)
+                       ∧ (∃e. (LABEL.edge_grp,l,l0,e)
+                                ∈ extractTrans m2 (SND y).frml
+                             ∧ ∀x.
+                               (LABEL,x) = h ∨ MEM (LABEL,x) qs ⇒
+                                 ∃node. lookup x m2.nodeInfo = SOME node
+                                      ∧ node.frml ∈ e)`
+                     suffices_by fs[]
+                >> qunabbrev_tac `addSingleEdge` >> Cases_on `h`
+                >> simp[]
+                >> `?nG. addEdge nId (q,r) m = SOME nG` by (
+                     simp[addEdge_def]
+                     >> Q.HO_MATCH_ABBREV_TAC `?nG. P ∧ A nG`
+                     >> `P ∧ (P ==> ?nG. A nG)` suffices_by fs[]
+                     >> qunabbrev_tac `P` >> qunabbrev_tac `A`
+                     >> rpt strip_tac
+                      >- (`MEM (nId,frml) (toAList g.nodeInfo)`
+                             by metis_tac[FIND_LEMM2]
+                          >> fs[MEM_toAList,domain_lookup]
+                          >> metis_tac[]
+                         )
+                      >- (`∃h. MEM (r,h) (toAList g.nodeInfo)` by metis_tac[]
+                          >> fs[MEM_toAList,domain_lookup]
+                          >> metis_tac[]
+                         )
+                      >- (`nId ∈ domain m.followers` by metis_tac[wfg_def]
+                          >> `?fol_o. lookup nId m.followers = SOME fol_o`
+                             by metis_tac[domain_lookup]
+                          >> fs[]
+                         )
+                 )
+                >> qexists_tac `nG` >> simp[]
+                >> `wfg nG` by metis_tac[addEdge_preserves_wfg]
+                >> POP_ASSUM mp_tac >> POP_ASSUM mp_tac
+                >> simp[addEdge_def] >> rpt strip_tac
+                >> Cases_on `m` >> fs[gfg_fn_updates]
+                >> fs[gfg_component_equality]
+                >> `?node. lookup r nG.nodeInfo = SOME node`
+                   by metis_tac[domain_lookup]
+                >> qexists_tac `e ∪ {node.frml}`
+                >> rpt strip_tac
+                >- (fs[extractTrans_def]
+                    >> qexists_tac `LABEL` >> simp[SET_EQ_SUBSET,SUBSET_DEF]
+                    >> rpt strip_tac
+                    >- (qunabbrev_tac `LABEL` >> fs[])
+                    >- (qunabbrev_tac `LABEL` >> fs[])
+                    >- (
+                     qexists_tac `suc` >> simp[] >> qexists_tac `sucId`
+                     >> simp[]
+                     >> Q.HO_MATCH_ABBREV_TAC `
+                         MEM (LABEL,sucId) (OPTION_TO_LIST M_L)`
+                     >> qabbrev_tac `M_L0 =
+                         do node <-
+                              findNode (λ(n',l). l.frml = (SND y).frml)
+                                       (gfg nG.nodeInfo s0 nG.preds nG.next);
+                            lookup node s0
+                         od`
+                     >> `IS_SOME M_L0`
+                           by metis_tac[MEM,OPTION_TO_LIST_def,
+                                        NOT_IS_SOME_EQ_NONE]
+                     >> `IS_SOME M_L` by (
+                         qunabbrev_tac `M_L` >> POP_ASSUM mp_tac
+                         >> qunabbrev_tac `M_L0` >> simp[IS_SOME_EXISTS]
+                         >> rpt strip_tac >> Cases_on `node' = nId`
+                         >- (qexists_tac `((q,r)::followers_old)`
+                             >> qexists_tac `nId` >> fs[findNode_def]
+                             >> metis_tac[lookup_insert]
+                            )
+                         >- (qexists_tac `x'` >> qexists_tac `node'`
+                             >> fs[findNode_def] >> metis_tac[lookup_insert]
+                            )
+                     )
+                     >> fs[IS_SOME_EXISTS,OPTION_TO_LIST_def]
+                     >> `MEM (label',sucId) x'` by metis_tac[OPTION_TO_LIST_def]
+                     >> qunabbrev_tac `M_L` >> qunabbrev_tac `M_L0` >> fs[]
+                     >> `node' = node''` by (
+                          Cases_on `nG` >> fs[findNode_def]
+                          >> rw[] >> metis_tac[SOME_11]
+                     )
+                     >> `LABEL = label'` by (
+                         qunabbrev_tac `LABEL`
+                         >> fs[theorem "edgeLabelAA_component_equality"]
+                     )
+                     >> rw[] >> Cases_on `node' = nId` >> fs[]
+                     >- (rw[]
+                         >> `x'' = (q,r)::followers_old`
+                            by metis_tac[lookup_insert,SOME_11]
+                         >> metis_tac[MEM]
+                        )
+                     >- (rw[] >> metis_tac[lookup_insert,SOME_11])
+                     )
+                    >- (rw[] >> qexists_tac `node` >> simp[] >> qexists_tac `r`
+                        >> simp[]
+                        >> Q.HO_MATCH_ABBREV_TAC `
+                            MEM (LABEL,r) (OPTION_TO_LIST M_L)`
+                        >> `IS_SOME M_L` by (
+                            simp[IS_SOME_EXISTS] >> qunabbrev_tac `M_L`
+                            >> qexists_tac `(q,r)::followers_old` >> fs[]
+                            >> qexists_tac `nId` >> fs[findNode_def]
+                            >> rpt strip_tac >>  metis_tac[lookup_insert]
+                         )
+                        >> fs[IS_SOME_EXISTS]
+                        >> `MEM (LABEL,r) x` suffices_by
+                              metis_tac[OPTION_TO_LIST_def,NOT_IS_SOME_EQ_NONE]
+                        >> qunabbrev_tac `M_L` >> fs[findNode_def]
+                        >> `node' = nId` by fs[] >> rw[]
+                        >> `q = LABEL` by metis_tac[] >> rw[]
+                        >> metis_tac[lookup_insert,SOME_11,MEM]
+                       )
+                    >- (Cases_on `x = node.frml` >> fs[]
+                        >> `LABEL = label'` by (
+                             qunabbrev_tac `LABEL`
+                             >> fs[theorem "edgeLabelAA_component_equality"]
+                         )
+                        >> rw[] >> qexists_tac `suc` >> fs[]
+                        >> qexists_tac `sucId` >> fs[]
+                        >> Q.HO_MATCH_ABBREV_TAC `
+                              MEM (LABEL,sucId) (OPTION_TO_LIST M_0)`
+                        >> qabbrev_tac `
+                            M_L =  do
+                                     node <- findNode
+                                              (λ(n,l). l.frml = (SND y).frml)
+                                              nG;
+                                     lookup node nG.followers
+                                    od`
+                        >> `IS_SOME M_L`
+                              by metis_tac[MEM,OPTION_TO_LIST_def,
+                                           NOT_IS_SOME_EQ_NONE]
+                        >> `IS_SOME M_0` by (
+                             qunabbrev_tac `M_L` >> POP_ASSUM mp_tac
+                             >> qunabbrev_tac `M_0` >> simp[IS_SOME_EXISTS]
+                             >> rpt strip_tac >> Cases_on `node' = nId`
+                             >- (qexists_tac `followers_old`
+                                 >> qexists_tac `nId` >> fs[findNode_def]
+                                )
+                             >- (qexists_tac `x` >> qexists_tac `node'`
+                                 >> fs[findNode_def] >> metis_tac[lookup_insert]
+                                )
+                         )
+                        >> fs[IS_SOME_EXISTS,OPTION_TO_LIST_def]
+                        >> `MEM (LABEL,sucId) x` by metis_tac[OPTION_TO_LIST_def]
+                        >> qunabbrev_tac `M_L` >> qunabbrev_tac `M_0` >> fs[]
+                        >> `node' = node''` by (
+                             Cases_on `nG` >> fs[findNode_def]
+                             >> rw[] >> metis_tac[SOME_11]
+                         )
+                        >> rw[]
+                        >> Cases_on `node' = nId` >> fs[]
+                        >- (rw[]
+                            >> `x = (q,r)::followers_old` by metis_tac[lookup_insert,SOME_11]
+                            >> `~(sucId = r)` by (
+                                `~(node = suc)` suffices_by metis_tac[SOME_11]
+                                >> fs[theorem "nodeLabelAA_component_equality"]
+                             )
+                            >> `~((LABEL,sucId) = (q,r))` by fs[]
+                            >> metis_tac[MEM]
+                           )
+                        >- (rw[] >> metis_tac[lookup_insert,SOME_11])
+                       )
+                   )
+                    >- fs[]
+                    >- (fs[] >> metis_tac[])
+                   )
+               )
+       >> `!qs.
 
 
 
